src/cbor/pulse/raw/CBOR.Pulse.API.Det.C.fst
@@ -4,6 +4,15 @@ module CBOR.Pulse.API.Det.C
 (* NOTE: this .fst file does not need anything from the Raw namespace,
 but it has been moved here to be hidden from verified clients. *)
 
+[@@pulse_unfold]
+let cbor_det_match = CBOR.Pulse.API.Det.Common.cbor_det_match
+
+let cbor_det_reset_perm = CBOR.Pulse.API.Det.Common.cbor_det_reset_perm
+
+let cbor_det_share = CBOR.Pulse.API.Det.Common.cbor_det_share
+
+let cbor_det_gather = CBOR.Pulse.API.Det.Common.cbor_det_gather
+
 fn cbor_det_validate
   (input: AP.ptr U8.t)
   (input_len: SZ.t)
@@ -78,6 +87,8 @@ ensures
   res
 }
 
+let cbor_det_size = CBOR.Pulse.API.Det.Common.cbor_det_size
+
 #restart-solver
 fn cbor_det_serialize
   (x: cbor_det_t)
@@ -91,7 +102,7 @@ returns res: SZ.t
 ensures
     (exists* v . cbor_det_match pm x y ** pts_to output v ** pure (
       SZ.v output_len == Seq.length v /\
-      cbor_det_serialize_postcond y res v
+      cbor_det_serialize_fits_postcond y res v
     ))
 {
   let ou = S.arrayptr_to_slice_intro output output_len;
@@ -117,14 +128,41 @@ fn cbor_det_impl_utf8_correct_from_array (_: unit) : cbor_det_impl_utf8_correct_
   res
 }
 
+let cbor_det_mk_simple_value = CBOR.Pulse.API.Det.Common.cbor_det_mk_simple_value
+let cbor_det_mk_int64 = CBOR.Pulse.API.Det.Common.cbor_det_mk_int64
+let cbor_det_mk_tagged = CBOR.Pulse.API.Det.Common.cbor_det_mk_tagged
+
 let cbor_det_mk_string_from_array (_: unit) =
-  mk_string_from_array (cbor_det_mk_string ())
+  mk_string_from_array (CBOR.Pulse.API.Det.Common.cbor_det_mk_string ())
 
 let cbor_det_mk_array_from_array (_: unit) =
-  mk_array_from_array (cbor_det_mk_array ())
+  mk_array_from_array (CBOR.Pulse.API.Det.Common.cbor_det_mk_array ())
+
+[@@pulse_unfold]
+let cbor_det_map_entry_match = CBOR.Pulse.API.Det.Common.cbor_det_map_entry_match
+
+let cbor_det_mk_map_entry = CBOR.Pulse.API.Det.Common.cbor_det_mk_map_entry
 
 let cbor_det_mk_map_from_array : mk_map_from_array_t cbor_det_match cbor_det_map_entry_match =
   mk_map_from_array (CBOR.Pulse.API.Base.mk_map_from_ref (CBOR.Pulse.API.Det.Type.dummy_cbor_det_t ()) (CBOR.Pulse.API.Det.Common.cbor_det_mk_map_gen ()))
+
+let cbor_det_equal = CBOR.Pulse.API.Det.Common.cbor_det_equal
+
+let cbor_det_major_type = CBOR.Pulse.API.Det.Common.cbor_det_major_type
+
+let cbor_det_read_simple_value = CBOR.Pulse.API.Det.Common.cbor_det_read_simple_value
+
+let cbor_det_elim_simple = CBOR.Pulse.API.Det.Common.cbor_det_elim_simple
+
+let cbor_det_read_uint64 = CBOR.Pulse.API.Det.Common.cbor_det_read_uint64
+
+let cbor_det_elim_int64 = CBOR.Pulse.API.Det.Common.cbor_det_elim_int64
+
+let cbor_det_get_string_length = CBOR.Pulse.API.Det.Common.cbor_det_get_string_length
+
+let cbor_det_get_tagged_tag = CBOR.Pulse.API.Det.Common.cbor_det_get_tagged_tag
+
+let cbor_det_get_tagged_payload = CBOR.Pulse.API.Det.Common.cbor_det_get_tagged_payload
 
 fn cbor_det_get_string
   (_: unit)
@@ -139,6 +177,50 @@ fn cbor_det_get_string
   Trade.trans _ _ (cbor_det_match p x y);
   res
 }
+
+let cbor_det_get_array_length = CBOR.Pulse.API.Det.Common.cbor_det_get_array_length
+
+[@@pulse_unfold]
+let cbor_det_array_iterator_match = CBOR.Pulse.API.Det.Common.cbor_det_array_iterator_match
+
+let cbor_det_array_iterator_start = CBOR.Pulse.API.Det.Common.cbor_det_array_iterator_start
+
+let cbor_det_array_iterator_is_empty = CBOR.Pulse.API.Det.Common.cbor_det_array_iterator_is_empty
+
+let cbor_det_array_iterator_length = CBOR.Pulse.API.Det.Common.cbor_det_array_iterator_length
+
+let cbor_det_array_iterator_next = CBOR.Pulse.API.Det.Common.cbor_det_array_iterator_next
+
+let cbor_det_array_iterator_truncate = CBOR.Pulse.API.Det.Common.cbor_det_array_iterator_truncate
+
+let cbor_det_array_iterator_share = CBOR.Pulse.API.Det.Common.cbor_det_array_iterator_share
+
+let cbor_det_array_iterator_gather = CBOR.Pulse.API.Det.Common.cbor_det_array_iterator_gather
+
+let cbor_det_get_array_item = CBOR.Pulse.API.Det.Common.cbor_det_get_array_item
+
+let cbor_det_get_map_length = CBOR.Pulse.API.Det.Common.cbor_det_get_map_length
+
+[@@pulse_unfold]
+let cbor_det_map_iterator_match = CBOR.Pulse.API.Det.Common.cbor_det_map_iterator_match
+
+let cbor_det_map_iterator_start = CBOR.Pulse.API.Det.Common.cbor_det_map_iterator_start
+
+let cbor_det_map_iterator_is_empty = CBOR.Pulse.API.Det.Common.cbor_det_map_iterator_is_empty
+
+let cbor_det_map_iterator_next = CBOR.Pulse.API.Det.Common.cbor_det_map_iterator_next
+
+let cbor_det_map_iterator_share = CBOR.Pulse.API.Det.Common.cbor_det_map_iterator_share
+
+let cbor_det_map_iterator_gather = CBOR.Pulse.API.Det.Common.cbor_det_map_iterator_gather
+
+let cbor_det_map_entry_key = CBOR.Pulse.API.Det.Common.cbor_det_map_entry_key
+
+let cbor_det_map_entry_value = CBOR.Pulse.API.Det.Common.cbor_det_map_entry_value
+
+let cbor_det_map_entry_share = CBOR.Pulse.API.Det.Common.cbor_det_map_entry_share
+
+let cbor_det_map_entry_gather = CBOR.Pulse.API.Det.Common.cbor_det_map_entry_gather
 
 fn cbor_det_map_get
   (_: unit)
