src/cbor/pulse/raw/CBOR.Pulse.API.Det.Common.fsti
@@ -70,108 +70,17 @@ val cbor_det_case_correct
 
 (* Validation, parsing and serialization *)
 
-noextract [@@noextract_to "krml"]
-let cbor_det_validate_post
-  (v: Seq.seq U8.t)
-  (res: SZ.t)
-: Tot prop
-=
-      if SZ.v res = 0
-      then (~ (exists v1 v2 . v == Spec.cbor_det_serialize v1 `Seq.append` v2))
-      else (exists v1 v2 . v == Spec.cbor_det_serialize v1 `Seq.append` v2 /\ SZ.v res == Seq.length (Spec.cbor_det_serialize v1))
-
-inline_for_extraction
-noextract [@@noextract_to "krml"]
-let cbor_det_validate_t
-=
-  (input: S.slice U8.t) ->
-  (#pm: perm) ->
-  (#v: Ghost.erased (Seq.seq U8.t)) ->
-  stt SZ.t
-    (pts_to input #pm v)
-    (fun res -> pts_to input #pm v ** pure (
-      cbor_det_validate_post v res
-    ))
-
 inline_for_extraction
 noextract [@@noextract_to "krml"]
 val cbor_det_validate (_: unit) : cbor_det_validate_t
 
-let cbor_det_parse_aux1
-  (v1: Spec.cbor)
-: Lemma
-  (let s = Spec.cbor_det_serialize v1 in s == s `Seq.append` Seq.empty)
-= Seq.append_empty_r (Spec.cbor_det_serialize v1)
-
 inline_for_extraction
 noextract [@@noextract_to "krml"]
-let cbor_det_parse_valid_t =
-  (input: S.slice U8.t) ->
-  (#pm: perm) ->
-  (#v: Ghost.erased (Seq.seq U8.t)) ->
-  stt cbor_det_t
-    (pts_to input #pm v ** pure (
-      exists v1 . Ghost.reveal v == Spec.cbor_det_serialize v1 /\ SZ.v (S.len input) == Seq.length (Spec.cbor_det_serialize v1)
-    ))
-    (fun res -> exists* v' .
-      cbor_det_match 1.0R res v' **
-      Trade.trade (cbor_det_match 1.0R res v') (pts_to input #pm v) ** pure (
-        Ghost.reveal v == Spec.cbor_det_serialize v'
-    ))
-
-inline_for_extraction
-noextract [@@noextract_to "krml"]
-val cbor_det_parse_valid (_: unit) : cbor_det_parse_valid_t
-
-let seq_length_append_l
-  (#t: Type)
-  (v1 v2: Seq.seq t)
-: Lemma
-  (Seq.slice (Seq.append v1 v2) 0 (Seq.length v1) == v1)
-= assert (Seq.slice (Seq.append v1 v2) 0 (Seq.length v1) `Seq.equal` v1)
+val cbor_det_parse_valid (_: unit) : cbor_det_parse_valid_t cbor_det_match
 
 module SU = Pulse.Lib.Slice.Util
 
-inline_for_extraction
-noextract [@@noextract_to "krml"]
-fn cbor_det_parse_full
-  (cbor_det_validate: cbor_det_validate_t)
-  (cbor_det_parse: cbor_det_parse_valid_t)
-: cbor_det_parse_t u#0 #_ cbor_det_match
-=
-  (input: S.slice U8.t)
-  (#pm: perm)
-  (#v: Ghost.erased (Seq.seq U8.t))
-{
-  let len = cbor_det_validate input;
-  Spec.cbor_det_parse_none_equiv v;
-  if (len = 0sz) {
-    fold (cbor_det_parse_post cbor_det_match input pm v None);
-    None #(cbor_det_t & S.slice U8.t)
-  } else {
-    Seq.lemma_split v (SZ.v len);
-    let input2, rem = SU.split_trade input len;
-    Classical.forall_intro_2 (seq_length_append_l #U8.t);
-    S.pts_to_len input2;
-    let res = cbor_det_parse input2;
-    Trade.trans_hyp_l _ _ _ (pts_to input #pm v);
-    fold (cbor_det_parse_post_some cbor_det_match input pm v res rem);
-    fold (cbor_det_parse_post cbor_det_match input pm v (Some (res, rem)));
-    Some (res, rem)
-  }
-}
-
-noextract [@@noextract_to "krml"]
-let cbor_det_size_post
-  (bound: SZ.t)
-  (y: Spec.cbor)
-  (res: SZ.t)
-: Tot prop
-=
-      let s = Seq.length (Spec.cbor_det_serialize y) in
-      (SZ.v res == 0 <==> s > SZ.v bound) /\
-      (SZ.v res > 0 ==> SZ.v res == s)
-
+inline_for_extraction noextract [@@noextract_to "krml"]
 val cbor_det_size
   (x: cbor_det_t)
   (bound: SZ.t)
@@ -183,17 +92,6 @@ val cbor_det_size
       cbor_det_size_post bound y res
     ))
 
-noextract [@@noextract_to "krml"]
-let cbor_det_serialize_postcond
-  (y: Spec.cbor)
-  (res: SZ.t)
-  (v: Seq.seq U8.t)
-: Tot prop
-=
-      let s = Spec.cbor_det_serialize y in
-      SZ.v res == Seq.length s /\
-      (exists v' . v `Seq.equal` (s `Seq.append` v'))
-
 inline_for_extraction
 noextract [@@noextract_to "krml"]
 val cbor_det_serialize
@@ -204,7 +102,7 @@ val cbor_det_serialize
 : stt SZ.t
     (exists* v . cbor_det_match pm x y ** pts_to output v ** pure (Seq.length (Spec.cbor_det_serialize y) <= SZ.v (S.len output)))
     (fun res -> exists* v . cbor_det_match pm x y ** pts_to output v ** pure (
-      cbor_det_serialize_postcond y res v
+      cbor_det_serialize_fits_postcond y res v
     ))
 
 inline_for_extraction
@@ -229,16 +127,20 @@ val cbor_det_serialize_map (_: unit) : cbor_det_serialize_map_t
 
 (* Constructors *)
 
+inline_for_extraction noextract [@@noextract_to "krml"]
 val cbor_det_mk_simple_value () : mk_simple_t cbor_det_match
+inline_for_extraction noextract [@@noextract_to "krml"]
 val cbor_det_mk_int64 () : mk_int64_t cbor_det_match
 inline_for_extraction noextract [@@noextract_to "krml"]
 val cbor_det_mk_string () : mk_string_t cbor_det_match
+inline_for_extraction noextract [@@noextract_to "krml"]
 val cbor_det_mk_tagged () : mk_tagged_t cbor_det_match
 inline_for_extraction noextract [@@noextract_to "krml"]
 val cbor_det_mk_array () : mk_array_t cbor_det_match
 
 val cbor_det_map_entry_match: perm -> cbor_det_map_entry_t -> Spec.cbor & Spec.cbor -> slprop
 
+inline_for_extraction noextract [@@noextract_to "krml"]
 val cbor_det_mk_map_entry () : mk_map_entry_t cbor_det_match cbor_det_map_entry_match
 
 inline_for_extraction noextract [@@noextract_to "krml"]
@@ -249,16 +151,25 @@ val cbor_det_utf8_correct () : impl_utf8_correct_t
 
 (* Destructors *)
 
+inline_for_extraction noextract [@@noextract_to "krml"]
 val cbor_det_equal () : equal_t cbor_det_match
+inline_for_extraction noextract [@@noextract_to "krml"]
 val cbor_det_major_type () : get_major_type_t cbor_det_match
+inline_for_extraction noextract [@@noextract_to "krml"]
 val cbor_det_read_simple_value () : read_simple_value_t cbor_det_match
+inline_for_extraction noextract [@@noextract_to "krml"]
 val cbor_det_elim_simple () : elim_simple_t cbor_det_match
+inline_for_extraction noextract [@@noextract_to "krml"]
 val cbor_det_read_uint64 () : read_uint64_t cbor_det_match
+inline_for_extraction noextract [@@noextract_to "krml"]
 val cbor_det_elim_int64 () : elim_int64_t cbor_det_match
+inline_for_extraction noextract [@@noextract_to "krml"]
 val cbor_det_get_string_length () : get_string_length_t cbor_det_match
 inline_for_extraction noextract [@@noextract_to "krml"]
 val cbor_det_get_string () : get_string_t cbor_det_match
+inline_for_extraction noextract [@@noextract_to "krml"]
 val cbor_det_get_tagged_tag () : get_tagged_tag_t cbor_det_match
+inline_for_extraction noextract [@@noextract_to "krml"]
 val cbor_det_get_tagged_payload () : get_tagged_payload_t cbor_det_match
 
 inline_for_extraction
@@ -269,42 +180,55 @@ inline_for_extraction
 noextract [@@noextract_to "krml"]
 let cbor_det_mk_simple_value' = mk_simple_value_trade _ (cbor_det_mk_simple_value ()) (cbor_det_elim_simple ())
 
+inline_for_extraction noextract [@@noextract_to "krml"]
 val cbor_det_get_array_length () : get_array_length_t cbor_det_match
 
 val cbor_det_array_iterator_match : perm -> cbor_det_array_iterator_t -> list Spec.cbor -> slprop
 
+inline_for_extraction noextract [@@noextract_to "krml"]
 val cbor_det_array_iterator_start () : array_iterator_start_t cbor_det_match cbor_det_array_iterator_match
 
+inline_for_extraction noextract [@@noextract_to "krml"]
 val cbor_det_array_iterator_is_empty () : array_iterator_is_empty_t cbor_det_array_iterator_match
 
+inline_for_extraction noextract [@@noextract_to "krml"]
 val cbor_det_array_iterator_length () : array_iterator_length_t cbor_det_array_iterator_match
 
+inline_for_extraction noextract [@@noextract_to "krml"]
 val cbor_det_array_iterator_next () : array_iterator_next_t cbor_det_match cbor_det_array_iterator_match
 
+inline_for_extraction noextract [@@noextract_to "krml"]
 val cbor_det_array_iterator_truncate () : array_iterator_truncate_t cbor_det_array_iterator_match
 
 val cbor_det_array_iterator_share () : share_t cbor_det_array_iterator_match
 
 val cbor_det_array_iterator_gather () : gather_t cbor_det_array_iterator_match
 
+inline_for_extraction noextract [@@noextract_to "krml"]
 val cbor_det_get_array_item () : get_array_item_t cbor_det_match
 
+inline_for_extraction noextract [@@noextract_to "krml"]
 val cbor_det_get_map_length () : get_map_length_t cbor_det_match
 
 val cbor_det_map_iterator_match : perm -> cbor_det_map_iterator_t -> list (Spec.cbor & Spec.cbor) -> slprop
 
+inline_for_extraction noextract [@@noextract_to "krml"]
 val cbor_det_map_iterator_start () : map_iterator_start_t cbor_det_match cbor_det_map_iterator_match
 
+inline_for_extraction noextract [@@noextract_to "krml"]
 val cbor_det_map_iterator_is_empty () : map_iterator_is_empty_t cbor_det_map_iterator_match
 
+inline_for_extraction noextract [@@noextract_to "krml"]
 val cbor_det_map_iterator_next () : map_iterator_next_t cbor_det_map_entry_match cbor_det_map_iterator_match
 
 val cbor_det_map_iterator_share () : share_t cbor_det_map_iterator_match
 
 val cbor_det_map_iterator_gather () : gather_t cbor_det_map_iterator_match
 
+inline_for_extraction noextract [@@noextract_to "krml"]
 val cbor_det_map_entry_key () : map_entry_key_t cbor_det_map_entry_match cbor_det_match
 
+inline_for_extraction noextract [@@noextract_to "krml"]
 val cbor_det_map_entry_value () : map_entry_value_t cbor_det_map_entry_match cbor_det_match
 
 val cbor_det_map_entry_share () : share_t cbor_det_map_entry_match
