src/cbor/pulse/raw/CBOR.Pulse.API.Det.C.Copy.fst
@@ -1,5 +1,6 @@
 module CBOR.Pulse.API.Det.C.Copy
 #lang-pulse
+friend CBOR.Pulse.API.Det.C
 friend CBOR.Pulse.API.Det.Common
 friend CBOR.Pulse.API.Det.Type
 friend CBOR.Spec.API.Format
@@ -23,7 +24,9 @@ let cbor_get_from_freeable x = Copy.Mkcbor_freeable?.cbor x
   (#v: _)
 {
   unfold (cbor_det_match p c v);
+  unfold (CBOR.Pulse.API.Det.Common.cbor_det_match p c v);
   let res = Copy.cbor_copy0 c;
+  fold (CBOR.Pulse.API.Det.Common.cbor_det_match p c v);
   fold (cbor_det_match p c v);
   Trade.rewrite_with_trade
     (Raw.cbor_match 1.0R res.cbor (SpecRaw.mk_det_raw_cbor v))
